theories/SimGlobal.v
@@ -1,0 +1,142 @@
+Require Import Coqlib.
+Require Import ITreelib.
+Require Import Universe.
+Require Import STS.
+Require Import Behavior.
+Require Import ModSem.
+Require Import Skeleton.
+Require Import PCM.
+Require Import Coq.Relations.Relation_Definitions.
+Require Import Relation_Operators.
+Require Import RelationPairs.
+
+Generalizable Variables E R A B C X Y Σ.
+
+Set Implicit Arguments.
+
+
+Section SIM.
+
+Context `{Σ: GRA.t}.
+
+Variable idx: Type.
+Variable ord: idx -> idx -> Prop.
+Hypothesis wf_ord: well_founded ord.
+
+Section TY.
+Context `{R: Type}.
+Inductive _simg (simg: idx -> relation (itree eventE R)) (i0: idx): relation (itree eventE R) :=
+| simg_ret
+    r
+  :
+    _simg simg i0 (Ret r) (Ret r)
+| simg_syscall
+    i1 ktr_src0 ktr_tgt0 fn m0 varg
+    (SIM: (eq ==> simg i1)%signature ktr_src0 ktr_tgt0)
+  :
+    _simg simg i0 (trigger (Syscall fn m0 varg) >>= ktr_src0) (trigger (Syscall fn m0 varg) >>= ktr_tgt0)
+
+
+
+| simg_tau
+    i1 itr_src0 itr_tgt0
+    (SIM: simg i1 itr_src0 itr_tgt0)
+  :
+    _simg simg i0 (tau;; itr_src0) (tau;; itr_tgt0)
+| simg_tauL
+    i1 itr_src0 itr_tgt0
+    (ORD: ord i1 i0)
+    (SIM: simg i1 itr_src0 itr_tgt0)
+  :
+    _simg simg i0 (tau;; itr_src0) (itr_tgt0)
+| simg_tauR
+    i1 itr_src0 itr_tgt0
+    (ORD: ord i1 i0)
+    (SIM: simg i1 itr_src0 itr_tgt0)
+  :
+    _simg simg i0 (itr_src0) (tau;; itr_tgt0)
+
+
+
+| simg_choose
+    i1 X_src X_tgt ktr_src0 ktr_tgt0
+    (SIM: forall x_tgt, exists x_src, simg i1 (ktr_src0 x_src) (ktr_tgt0 x_tgt))
+  :
+    _simg simg i0 (trigger (Choose X_src) >>= ktr_src0) (trigger (Choose X_tgt) >>= ktr_tgt0)
+| simg_chooseL
+    i1 X ktr_src0 itr_tgt0
+    (ORD: ord i1 i0)
+    (SIM: exists x, simg i1 (ktr_src0 x) itr_tgt0)
+  :
+    _simg simg i0 (trigger (Choose X) >>= ktr_src0) (itr_tgt0)
+| simg_chooseR
+    i1 X itr_src0 ktr_tgt0
+    (ORD: ord i1 i0)
+    (SIM: forall x, simg i1 itr_src0 (ktr_tgt0 x))
+  :
+    _simg simg i0 (itr_src0) (trigger (Choose X) >>= ktr_tgt0)
+
+
+
+| simg_take
+    i1 X_src X_tgt ktr_src0 ktr_tgt0
+    (SIM: forall x_src, exists x_tgt, simg i1 (ktr_src0 x_src) (ktr_tgt0 x_tgt))
+  :
+    _simg simg i0 (trigger (Take X_src) >>= ktr_src0) (trigger (Take X_tgt) >>= ktr_tgt0)
+| simg_takeL
+    i1 X ktr_src0 itr_tgt0
+    (ORD: ord i1 i0)
+    (SIM: forall x, simg i1 (ktr_src0 x) itr_tgt0)
+  :
+    _simg simg i0 (trigger (Take X) >>= ktr_src0) (itr_tgt0)
+| simg_takeR
+    i1 X itr_src0 ktr_tgt0
+    (ORD: ord i1 i0)
+    (SIM: exists x, simg i1 itr_src0 (ktr_tgt0 x))
+  :
+    _simg simg i0 (itr_src0) (trigger (Take X) >>= ktr_tgt0)
+.
+
+Definition simg: idx -> relation (itree eventE R) := paco3 _simg bot3.
+
+Lemma simg_mon: monotone3 _simg.
+Proof.
+  ii. inv IN; try (by econs; et).
+  - econs; et. ii. eapply LE; et.
+  - econs; et. ii. hexploit SIM; et. i; des. esplits; et.
+  - des. econs; et.
+  - econs; et. ii. hexploit SIM; et. i; des. esplits; et.
+  - des. econs; et.
+Qed.
+End TY.
+
+
+(*** TODO: for bind rule, take a look at "respectful" thing again. ***)
+
+
+
+
+
+
+Definition resum_itr E F `{E -< F}: itree E ~> itree F := fun _ itr => interp (fun _ e => trigger e) itr.
+
+Variable md_src md_tgt: Mod.t.
+Let ms_src: ModSem.t := md_src.(Mod.enclose).
+Let ms_tgt: ModSem.t := md_tgt.(Mod.enclose).
+Let sim_fnsem: relation (string * (list val -> itree Es val)) :=
+  fun '(fn_src, fsem_src) '(fn_tgt, fsem_tgt) =>
+    (<<NAME: fn_src = fn_tgt>>) /\
+    (<<SEM: forall varg, exists itr_src itr_tgt,
+          (<<SRC: fsem_src varg = resum_itr itr_src>>) /\
+          (<<TGT: fsem_tgt varg = resum_itr itr_tgt>>) /\
+          (<<SIM: exists i0, simg i0 itr_src itr_tgt>>)>>)
+.
+
+Hypothesis (SIM: Forall2 sim_fnsem ms_src.(ModSem.fnsems) ms_tgt.(ModSem.fnsems)).
+
+Theorem adequacy_global: Beh.of_program (Mod.interp md_tgt) <1= Beh.of_program (Mod.interp md_src).
+Proof.
+  admit "TODO".
+Qed.
+
+End SIM.
